List selector as mfun

theories/ListSelector.v
@@ -6,12 +6,12 @@ Import ListNotations.
 From Hammer Require Import
   Tactics.
 
-Require Import Setoids.
+Require Import Setoids Multifunction.
 
 Open Scope slot_scope.
 
 Section defn.
-  Context {A : Type}.
+  Context {A : Type} `{Hsetoid : Setoid A}.
 
   Definition Pick (l : list A) a (l' : list A) : Prop :=
     Add a l' l.
@@ -76,6 +76,30 @@ Section defn.
     induction l1; intros l2 Hl2; sauto.
   Qed.
 
+  Program Definition pick_mfun : @MFunRet A (list A) Hsetoid (setoid_permutation _) :=
+    {| morphism l ret :=
+        let (a, l') := ret in
+        Pick l a l'
+    |}.
+  Next Obligation.
+    eapply pick_equiv in H; eauto.
+    destruct H as [l2' [Hal2' Hl2']].
+    exists (a, l2'); sauto.
+  Qed.
+
+  Definition pick_cons_mfun (a : A) : @MFun (list A) (list A)
+                                        (setoid_permutation _)
+                                        (setoid_permutation _).
+    refine (pure (cons a) _).
+    intros l l' Hll'.
+    now constructor.
+  Defined.
+
+  Lemma pick_cons_cons_commute (a b : A) : commute (pick_cons_mfun a) (pick_cons_mfun b).
+  Proof.
+    unfold pick_cons_mfun. apply pure_commutativity.
+    intros l. constructor.
+  Qed.
 End defn.
 
 Ltac rev_pick_cons :=
